\documentclass[a4paper,12pt]{article}
\usepackage[T1]{fontenc}
\usepackage[utf8]{inputenc}
\usepackage[polish]{babel}
\let\lll\undefined
\usepackage{amssymb}
\usepackage{amsthm}
\usepackage{times}
\usepackage{anysize}
\usepackage{enumitem}
\usepackage{textcomp}

\sloppy


\begin{document} 
	\textbf{Twierdzenie.} \textit{Jeżeli} $ \lim\limits_{n \to \infty} a_n = a i \lim_{n \to \infty} b_n = +\infty, to:$
	\begin{enumerate}[label={\arabic*°}]
		
		\item \begin{equation}
\lim_{n \to \infty}(a_n + b_n) = +\infty,
		\end{equation}
		\item $\lim_{n \to \infty}(a_n * b_n) = $
	$\left \{	
	\begin{array}{ccc}
	+\infty, & gdy & a>0,\\
	-\infty, & gdy & a<0,
	\end{array}
		\right .
	$
	\item $\lim_{n \to \infty}\frac{a_n}{b_n} = 0, przy b_n \neq 0 dla n \in \mathbb{N},$
	\item $	\lim_{n \to \infty}\frac{a_n}{b_n} = 
	\left \{	
	\begin{array}{ccc}
		+\infty, & gdy & a>0,\\
		-\infty, & gdy & a<0,
	\end{array}
	\right . przy załóżeniu że a_n \neq 0 dla n \in \mathbb{N}.$
\end{enumerate}
\end{document}